src/ElimFuncComp3.v
@@ -1,0 +1,405 @@
+Require Import Common Monads.
+Require Import Metadata.
+Require String.
+Require ElimFunc2 ElimFunc3.
+Require Import ListLemmas.
+
+Require Import Psatz.
+
+Module A := ElimFunc2.
+Module B := ElimFunc3.
+
+(* Additional alias - "Syntax", for common AST definitions *)
+Module S := ElimFunc2.
+
+
+Definition compile :=
+    let fix go e :=
+        let fix go_list es :=
+            match es with
+            | [] => []
+            | e :: es => go e :: go_list es
+            end in
+        let fix go_pair p :=
+            let '(e, r) := p in (go e, r) in
+        let fix go_list_pair ps :=
+            match ps with
+            | [] => []
+            | p :: ps => go_pair p :: go_list_pair ps
+            end in
+        match e with
+        | S.Arg => S.Arg
+        | S.UpVar n => S.UpVar n
+        | S.Call f a => S.Call (go f) (go a)
+        | S.Constr tag args => S.Constr tag (go_list args)
+        | S.ElimBody rec cases =>
+            S.ElimBody (go rec) (S.shift_list_pair (go_list_pair cases))
+        | S.Close fname free => S.Close fname (go_list free)
+        end in go.
+
+Definition compile_list :=
+    let go := compile in
+    let fix go_list es :=
+        match es with
+        | [] => []
+        | e :: es => go e :: go_list es
+        end in go_list.
+
+Definition compile_pair :=
+    let go := compile in
+    let fix go_pair (p : A.expr * A.rec_info) :=
+        let '(e, r) := p in (go e, r) in go_pair.
+
+Definition compile_list_pair :=
+    let go_pair := compile_pair in
+    let fix go_list_pair ps :=
+        match ps with
+        | [] => []
+        | p :: ps => go_pair p :: go_list_pair ps
+        end in go_list_pair.
+
+Ltac refold_compile :=
+    fold compile_list in *;
+    fold compile_pair in *;
+    fold compile_list_pair in *.
+
+
+Definition compile_cu (cu : list S.expr * list metadata) : list S.expr * list metadata :=
+    let '(exprs, metas) := cu in
+    let exprs' := compile_list exprs in
+    (exprs', metas).
+
+
+Lemma compile_list_Forall : forall aes bes,
+    compile_list aes = bes ->
+    Forall2 (fun a b => compile a = b) aes bes.
+induction aes; destruct bes; intros0 Hcomp; simpl in Hcomp; try discriminate.
+- constructor.
+- invc Hcomp. eauto.
+Qed.
+
+Lemma compile_list_length : forall es,
+    length (compile_list es) = length es.
+intros. induction es.
+- reflexivity.
+- simpl. f_equal. eauto.
+Qed.
+
+Lemma compile_list_pair_length : forall es,
+    length (compile_list_pair es) = length es.
+intros. induction es.
+- reflexivity.
+- simpl. f_equal. eauto.
+Qed.
+
+
+
+
+
+
+Definition on_fst (P : S.expr -> S.expr -> Prop) (ap bp : S.expr * S.rec_info) :=
+    P (fst ap) (fst bp) /\ snd ap = snd bp.
+
+Inductive I_expr (AE : S.env) (BE : S.env) : S.expr -> S.expr -> Prop :=
+| IArg : I_expr AE BE S.Arg S.Arg
+| IUpVar : forall n, I_expr AE BE (S.UpVar n) (S.UpVar n)
+| ICall : forall af aa bf ba,
+        I_expr AE BE af bf ->
+        I_expr AE BE aa ba ->
+        I_expr AE BE (S.Call af aa) (S.Call bf ba)
+| IConstr : forall tag aargs bargs,
+        Forall2 (I_expr AE BE) aargs bargs ->
+        I_expr AE BE (S.Constr tag aargs) (S.Constr tag bargs)
+| IElimBody : forall arec acases brec bcases,
+        I_expr AE BE arec brec ->
+        Forall2 (on_fst (I_expr AE BE)) (S.shift_list_pair acases) bcases ->
+        I_expr AE BE (S.ElimBody arec acases) (S.ElimBody brec bcases)
+| IClose : forall fname afree bfree,
+        Forall2 (I_expr AE BE) afree bfree ->
+        I_expr AE BE (S.Close fname afree) (S.Close fname bfree)
+.
+
+Definition I_pair AE BE := on_fst (I_expr AE BE).
+
+Inductive I (AE : S.env) (BE : S.env) : A.state -> B.state -> Prop :=
+| IRun : forall ae al ak be bl bk,
+        S.elim_body_placement ae ->
+        I_expr AE BE ae be ->
+        Forall2 (I_expr AE BE) al bl ->
+        Forall S.value al ->
+        Forall S.value bl ->
+        (forall av bv,
+            S.value av ->
+            S.value bv ->
+            I_expr AE BE av bv ->
+            I AE BE (ak av) (bk bv)) ->
+        I AE BE (A.Run ae al ak) (B.Run be bl bk)
+
+| IRunCase : forall ae al ak be bl bk  tag args,
+        Forall S.value args ->
+        S.no_elim_body ae ->
+        I_expr AE BE (S.shift ae) be ->
+        Forall2 (I_expr AE BE) al bl ->
+        Forall S.value al ->
+        Forall S.value bl ->
+        (forall av bv,
+            S.value av ->
+            S.value bv ->
+            I_expr AE BE av bv ->
+            I AE BE (ak av) (bk bv)) ->
+        I AE BE (A.Run ae al ak) (B.Run be (S.Constr tag args :: bl) bk)
+
+| IStop : forall ae be,
+        I_expr AE BE ae be ->
+        I AE BE (A.Stop ae) (B.Stop be).
+
+
+
+Lemma no_elim_body_placement : forall e,
+    S.no_elim_body e ->
+    S.elim_body_placement e.
+unfold S.elim_body_placement.
+destruct e; intro; eauto.
+on (S.no_elim_body _), invc.
+Qed.
+
+Lemma value_no_elim_body : forall e,
+    S.value e ->
+    S.no_elim_body e.
+induction e using S.expr_ind''; intros0 Hval; invc Hval.
+- simpl. S.refold_no_elim_body. rewrite S.no_elim_body_list_Forall.
+  list_magic_on (args, tt).
+- simpl. S.refold_no_elim_body. rewrite S.no_elim_body_list_Forall.
+  list_magic_on (free, tt).
+Qed.
+
+Lemma shift_list_pair_Forall2 : forall AE BE aps bps,
+    Forall2 (fun ap bp => on_fst (I_expr AE BE) (S.shift_pair ap) bp) aps bps <->
+    Forall2 (on_fst (I_expr AE BE)) (S.shift_list_pair aps) bps.
+induction aps; split; intro HH; invc HH;
+simpl in *; S.refold_shift.
+
+- constructor.
+- constructor.
+- constructor; eauto. rewrite <- IHaps. auto.
+- constructor; eauto. rewrite -> IHaps. auto.
+Qed.
+
+Lemma shift_I_expr : forall AE BE be ae,
+    I_expr AE BE ae be ->
+    I_expr AE BE (S.shift ae) (S.shift be).
+intros AE BE.
+induction be using A.expr_rect_mut with
+    (Pl := fun bes => forall aes,
+        Forall2 (I_expr AE BE) aes bes ->
+        Forall2 (I_expr AE BE) (S.shift_list aes) (S.shift_list bes))
+    (Pp := fun bp => forall ap,
+        I_pair AE BE ap bp ->
+        I_pair AE BE (S.shift_pair ap) (S.shift_pair bp))
+    (Plp := fun bps => forall aps,
+        Forall2 (I_pair AE BE) aps bps ->
+        Forall2 (I_pair AE BE) (S.shift_list_pair aps) (S.shift_list_pair bps));
+intros0 II; try solve [invc II; constructor; eauto].
+
+- destruct ap. unfold I_pair, on_fst in *. simpl. firstorder eauto.
+Qed.
+
+Lemma shift_list_pair_I_pair : forall AE BE aps bps,
+    Forall2 (I_pair AE BE) aps bps ->
+    Forall2 (I_pair AE BE) (S.shift_list_pair aps) (S.shift_list_pair bps).
+induction aps; intros0 Hfa; invc Hfa;
+simpl in *; S.refold_shift.
+- constructor.
+- constructor; eauto.
+  destruct a, y. unfold I_pair, on_fst in *. firstorder eauto.
+  simpl in *. eauto using shift_I_expr.
+Qed.
+
+
+Theorem compile_I_expr : forall AE BE ae be,
+    compile ae = be ->
+    I_expr AE BE ae be.
+intros AE BE.
+induction ae using A.expr_rect_mut with
+    (Pl := fun aes => forall bes,
+        compile_list aes = bes ->
+        Forall2 (I_expr AE BE) aes bes)
+    (Pp := fun ap => forall bp,
+        compile_pair ap = bp ->
+        I_pair AE BE ap bp)
+    (Plp := fun aps => forall bps,
+        compile_list_pair aps = bps ->
+        Forall2 (I_pair AE BE) aps bps);
+intros0 Hcomp;
+simpl in Hcomp; refold_compile; try rewrite <- Hcomp in *;
+try solve [eauto | constructor; eauto].
+
+- (* ElimBody *)
+  constructor; eauto.
+  eapply shift_list_pair_I_pair. eauto.
+Qed.
+
+
+
+Lemma I_expr_value : forall AE BE a b,
+    I_expr AE BE a b ->
+    S.value a ->
+    S.value b.
+induction a using S.expr_ind''; intros0 II Aval; invc Aval; invc II.
+- constructor. list_magic_on (args, (bargs, tt)).
+- constructor. list_magic_on (free, (bfree, tt)).
+Qed.
+Hint Resolve I_expr_value.
+
+Lemma I_expr_value' : forall AE BE b a,
+    I_expr AE BE a b ->
+    S.value b ->
+    S.value a.
+induction b using S.expr_ind''; intros0 II Bval; invc Bval; invc II.
+- constructor. list_magic_on (args, (aargs, tt)).
+- constructor. list_magic_on (free, (afree, tt)).
+Qed.
+
+Lemma I_expr_not_value : forall AE BE a b,
+    I_expr AE BE a b ->
+    ~S.value a ->
+    ~S.value b.
+intros. intro. fwd eapply I_expr_value'; eauto.
+Qed.
+Hint Resolve I_expr_not_value.
+
+Lemma I_expr_not_value' : forall AE BE a b,
+    I_expr AE BE a b ->
+    ~S.value b ->
+    ~S.value a.
+intros. intro. fwd eapply I_expr_value; eauto.
+Qed.
+
+
+Lemma shift_value_eq : forall e,
+    S.value e ->
+    S.shift e = e.
+induction e using S.expr_rect_mut with
+    (Pl := fun e =>
+        Forall S.value e ->
+        S.shift_list e = e)
+    (Pp := fun p =>
+        S.value (fst p) ->
+        S.shift_pair p = p)
+    (Plp := fun ps =>
+        Forall (fun p => S.value (fst p)) ps ->
+        S.shift_list_pair ps = ps);
+intros0 Hval; try solve [invc Hval];
+simpl; S.refold_shift.
+
+- invc Hval. f_equal. eauto.
+- invc Hval. f_equal. eauto.
+
+- reflexivity.
+- invc Hval. f_equal; eauto.
+
+- simpl in Hval. f_equal; eauto.
+
+- reflexivity.
+- invc Hval. f_equal; eauto.
+Qed.
+
+Lemma shift_value : forall e,
+    S.value e ->
+    S.value (S.shift e).
+intros. rewrite shift_value_eq; eauto.
+Qed.
+Hint Resolve shift_value.
+
+Lemma shift_not_value : forall e,
+    ~ S.value e ->
+    ~ S.value (S.shift e).
+induction e using S.expr_rect_mut with
+    (Pl := fun e =>
+        Forall (fun e => ~ S.value e) e ->
+        Forall (fun e => ~ S.value e) (S.shift_list e))
+    (Pp := fun p =>
+        ~ S.value (fst p) ->
+        ~ S.value (fst (S.shift_pair p)))
+    (Plp := fun ps =>
+        Forall (fun p => ~ S.value (fst p)) ps ->
+        Forall (fun p => ~ S.value (fst p)) (S.shift_list_pair ps));
+intros0 Hval; simpl; S.refold_shift; try solve [inversion 1].
+
+- contradict Hval. invc Hval. constructor.
+  admit. (* TODO *)
+- contradict Hval. invc Hval. constructor.
+  admit. (* TODO *)
+
+- constructor.
+- invc Hval. constructor; eauto.
+
+- simpl in Hval. eauto.
+
+- constructor.
+- invc Hval. constructor; eauto.
+Admitted.
+Hint Resolve shift_not_value.
+
+
+
+
+Ltac solve_value :=
+    eapply Forall_nth_error + eapply Forall2_nth_error;
+    cycle 1; solve [eauto].
+
+Theorem I_sim : forall AE BE a a' b,
+    compile_list AE = BE ->
+    I AE BE a b ->
+    A.sstep AE a a' ->
+    exists b',
+        B.sstep BE b b' /\
+        I AE BE a' b'.
+
+destruct a as [ae al ak | ae];
+intros0 Henv II Astep; [ | solve [invc Astep] ].
+
+destruct ae; inv Astep; invc II; try on (I_expr _ _ _ _), invc.
+
+
+- assert (HH : exists bv, nth_error bl 0 = Some bv) by admit.
+    destruct HH as [bv ?].
+  eexists. split. eapply B.SArg; eauto.
+  on _, eapply_; solve_value.
+
+- assert (HH : exists bv, nth_error bl 0 = Some bv) by admit.
+    destruct HH as [bv ?].
+  eexists. split. eapply B.SUpVar; eauto.
+  on _, eapply_; solve_value.
+
+
+- assert (HH : exists bv, nth_error bl (S n) = Some bv) by admit.
+    destruct HH as [bv ?].
+  eexists. split. eapply B.SUpVar; eauto.
+  on _, eapply_; solve_value.
+
+- assert (HH : exists bv, nth_error bl (S n) = Some bv) by admit.
+    destruct HH as [bv ?].
+  eexists. split. eapply B.SUpVar; eauto.
+  on _, eapply_; solve_value.
+
+
+- eexists. split. eapply B.SCallL; eauto.
+  constructor; eauto.
+    { simpl in *. eapply no_elim_body_placement; firstorder. }
+  intros. constructor; eauto.
+    { simpl in *. split; eauto using value_no_elim_body. firstorder. }
+  constructor; eauto.
+
+- eexists. split. eapply B.SCallL; eauto.
+  admit.
+  (*
+  constructor; eauto.
+    { simpl in *. eapply no_elim_body_placement; firstorder. }
+  intros. constructor; eauto.
+    { simpl in *. split; eauto using value_no_elim_body. firstorder. }
+  constructor; eauto.
+*)
+
+Admitted.
+
